Eval tactic working

SkLean/EvalTactic.lean
@@ -6,63 +6,99 @@ import Lean.Expr
 open Lean Meta Qq
 open PrettyPrinter
 
+declare_syntax_cat skmexprquot
+syntax "K"                                                             : skmexprquot
+syntax "S"                                                             : skmexprquot
+syntax "M"                                                             : skmexprquot
+syntax "(" skmexprquot skmexprquot ")"                                 : skmexprquot
+syntax ident                                                           : skmexprquot
+syntax "#" term                                                        : skmexprquot
+syntax "(" skmexprquot ")"                                             : skmexprquot
+
+syntax " << " skmexprquot " >> "                                      : term
+syntax "SKM`[ " skmexprquot " ] "                                      : term
+
+macro_rules
+  | `(SKM`[ $e:skmexprquot ]) => `(<< $e >>)
+
+macro_rules
+  | `(<< K >>)                           => `(Lean.Expr.const `Expr.k [])
+  | `(<< S >>)                           => `(Lean.Expr.const `Expr.s [])
+  | `(<< M >>)                           => `(Lean.Expr.const `Expr.m [])
+  | `(<< $e:ident >>)                    => `($e)
+  | `(<< ($e₁:skmexprquot $e₂:skmexprquot) >>)   => `(Lean.Expr.app
+      (Lean.Expr.app (Lean.Expr.const `Expr.call []) << $e₁ >>)
+    << $e₂ >>)
+  | `(<< ($e:skmexprquot) >>)            => `(<<$e>>)
+
 -- Closes a goal of the form `beta_eq e₁ e₂` by recursively evaluating the expression
 partial def eval_to (from_e : Lean.Expr) (to_e : Option Lean.Expr) : OptionT MetaM $ List Lean.Expr := do
   if (← (to_e.map $ isDefEq from_e).getD (pure false)) then
     pure []
   else match from_e with
-    | (.app (.app (.const `SkLean.Ast3.Expr.k []) x) _y) =>
+    | SKM`[((K x) _y)] =>
       pure $ ([
-        (Lean.Expr.const `SkLean.Ast3.beta_eq.eval []),
-        (Lean.Expr.const `SkLean.Ast3.is_eval_once.k []),
+        (Lean.Expr.const `beta_eq.eval []),
+        (Lean.Expr.const `is_eval_once.k []),
       ]) ++ (← eval_to x to_e)
-    | (.app (.app (.app (.const `SkLean.Ast3.Expr.s []) x) y) z) =>
+    | SKM`[(((S x) y) z)] =>
       pure $ ([
-        (Lean.Expr.const `SkLean.Ast3.beta_eq.eval []),
-        (Lean.Expr.const `SkLean.Ast3.is_eval_once.s []),
-      ]) ++ (← eval_to (.app (.app x z) (.app y z))  to_e)
-    | (.app (.const `SkLean.Ast3.Expr.m []) (.const `SkLean.Ast3.Expr.k [])) =>
-      let e' ← OptionT.mk (pure $ (← getConstInfo `SkLean.Ast3.t_k).value?)
+        (Lean.Expr.const `beta_eq.eval []),
+        (Lean.Expr.const `is_eval_once.s []),
+      ]) ++ (← eval_to SKM`[((x z) (y z))] to_e)
+    | SKM`[(M K)] =>
+      let e' ← OptionT.mk (pure $ (← getConstInfo `t_k).value?)
 
       pure $ ([
-        (Lean.Expr.const `SkLean.Ast3.beta_eq.eval []),
-        (Lean.Expr.const `SkLean.Ast3.is_eval_once.m_k []),
+        (Lean.Expr.const `beta_eq.eval []),
+        (Lean.Expr.const `is_eval_once.m_k []),
       ]) ++ (← eval_to e' to_e)
-    | (.app (.const `SkLean.Ast3.Expr.m []) (.const `SkLean.Ast3.Expr.m [])) =>
-      let e' ← OptionT.mk (pure $ (← getConstInfo `SkLean.Ast3.t_m).value?)
+    | SKM`[(M M)] =>
+      let e' ← OptionT.mk (pure $ (← getConstInfo `t_m).value?)
 
       pure $ ([
-        (Lean.Expr.const `SkLean.Ast3.beta_eq.eval []),
-        (Lean.Expr.const `SkLean.Ast3.is_eval_once.m_m []),
+        (Lean.Expr.const `beta_eq.eval []),
+        (Lean.Expr.const `is_eval_once.m_m []),
       ]) ++ (← eval_to e' to_e)
-    | (.app (.const `SkLean.Ast3.Expr.m []) (.const `SkLean.Ast3.Expr.s [])) =>
-      let e' ← OptionT.mk (pure $ (← getConstInfo `SkLean.Ast3.t_s).value?)
+    | SKM`[(M S)] =>
+      let e' ← OptionT.mk (pure $ (← getConstInfo `t_s).value?)
 
       pure $ ([
-        (Lean.Expr.const `SkLean.Ast3.beta_eq.eval []),
-        (Lean.Expr.const `SkLean.Ast3.is_eval_once.m_s []),
+        (Lean.Expr.const `beta_eq.eval []),
+        (Lean.Expr.const `is_eval_once.m_s []),
       ]) ++ (← eval_to e' to_e)
-    | (.app (.const `SkLean.Ast3.Expr.m []) (.app (.const `SkLean.Ast3.Expr.m []) (.app (.app (.const `SkLean.Ast3.Expr.call []) e₁) e₂))) =>
-      let t_out ← OptionT.mk (pure $ (← getConstInfo `SkLean.Ast3.t_out).value?)
-      let e' := (Lean.Expr.app (.app (Lean.Expr.const `SkLean.Ast3.Expr.call []) t_out) (.app (.app (.const `SkLean.Ast3.Expr.m []) e₁) e₂))
+    | SKM`[(M (e₁ e₂))] =>
+      let t_out ← OptionT.mk (pure $ (← getConstInfo `t_out).value?)
+      let e' := SKM`[(t_out ((M e₁) e₂))]
 
       pure $ ([
-        (Lean.Expr.const `SkLean.Ast3.beta_eq.eval []),
-        (Lean.Expr.const `SkLean.Ast3.is_eval_once.m_call [])
+        (Lean.Expr.const `beta_eq.eval []),
+        (Lean.Expr.const `is_eval_once.m_call [])
       ]) ++ (← eval_to e' to_e)
-    | (.app lhs rhs) =>
-      pure $ (Lean.Expr.const `SkLean.Ast3.beta_eq.left []) :: (← eval_to lhs none)
+    | SKM`[(lhs rhs)] =>
+      pure $ (Lean.Expr.const `beta_eq.left []) :: (← eval_to lhs none)
     | _ => pure []
+
+def parse_beta_eq_call (e : Lean.Expr) : OptionT MetaM $ Lean.Expr × Lean.Expr := do
+  let e ← whnf e
+  match e with
+    | .app (.app (.const `beta_eq []) from_e) to_e =>
+      pure $ ⟨from_e, to_e⟩
+    | _ =>
+      OptionT.mk (pure .none)
 
 syntax "eval_to" ( term ) : tactic
 
 open Elab Tactic
 elab_rules : tactic
   | `(tactic| eval_to $e) => do
+    let e' ← (((do
     let goal      ← getMainGoal
     let goal_e := (← Term.getMVarDecl goal).type
+    let ⟨from_e, _⟩ ← OptionT.mk (pure $ ← liftMetaM $ parse_beta_eq_call goal_e)
+    let to_e ← elabTerm e none
 
-    let exprs ← liftMetaM (OptionT.run $ eval_to goal_e (← elabTerm e none))
+    let exprs ← liftMetaM $ eval_to from_e to_e
 
     match exprs with
       | Option.some exprs =>
@@ -70,6 +106,10 @@ elab_rules : tactic
           let e_stx ← delab e
           evalTactic (← `(tactic| apply $e_stx))
       | .none =>
-        return ()
+        return ()) : OptionT TacticM Unit)
+          |> OptionT.run)
+    pure $ e'.getD ()
 
+example : beta_eq SKM[((K x) y)] x := by
+  eval_to x
 
