SkLean/Proof.lean
@@ -1,0 +1,6 @@
+import SkLean.Ast3
+import SkLean.EvalTactic
+
+example : beta_eq SKM[((K x) y)] x := by
+  eval_to x
+  
